Optimization correctness.

opt.v
@@ -1,4 +1,4 @@
-From stdpp Require Import base gmap.
+From stdpp Require Import base gmap ssreflect strings.
 From introduction Require Import imp.
 
 Definition cp_add e1 e2 :=
@@ -79,3 +79,259 @@ Fixpoint cp_com c :=
   | If e c1 c2 => cp_if (cp_expr e) (cp_com c1) (cp_com c2)
   | While e c => cp_while (cp_expr e) (cp_com c)
   end.
+
+Inductive cp_add_spec : expr -> expr -> expr -> Prop :=
+| CpAdd1 n1 n2 : cp_add_spec (Num n1) (Num n2) (Num (n1 + n2))
+| CpAdd2 e : cp_add_spec (Num 0) e e
+| CpAdd3 e : cp_add_spec e (Num 0) e
+| CpAdd4 e1 e2 : cp_add_spec e1 e2 (Binop Add e1 e2).
+
+Lemma cp_addP e1 e2 : cp_add_spec e1 e2 (cp_add e1 e2).
+Proof.
+case: e1 => [x1|[|n1]|b1 e11 e12] /=;
+case: e2 => [x2|[|n2]|b2 e21 e22] /=;
+eauto using cp_add_spec.
+Qed.
+
+Inductive cp_mul_spec : expr -> expr -> expr -> Prop :=
+| CpMul1 n1 n2 : cp_mul_spec (Num n1) (Num n2) (Num (n1 * n2))
+| CpMul2 e : cp_mul_spec (Num 0) e (Num 0)
+| CpMul3 e : cp_mul_spec e (Num 0) (Num 0)
+| CpMul4 e : cp_mul_spec (Num 1) e e
+| CpMul5 e : cp_mul_spec e (Num 1) e
+| CpMul6 e1 e2 : cp_mul_spec e1 e2 (Binop Mul e1 e2).
+
+Lemma cp_mulP e1 e2 : cp_mul_spec e1 e2 (cp_mul e1 e2).
+Proof.
+case: e1 => [x1|[|[|n1]]|b1 e11 e12];
+case: e2 => [x2|[|[|n2]]|b2 e21 e22];
+eauto using cp_mul_spec.
+Qed.
+
+Inductive cp_sub_spec : expr -> expr -> expr -> Prop :=
+| CpSub1 n1 n2 : cp_sub_spec (Num n1) (Num n2) (Num (n1 - n2))
+| CpSub2 e : cp_sub_spec (Num 0) e (Num 0)
+| CpSub3 e : cp_sub_spec e (Num 0) e
+| CpSub4 e1 e2 : cp_sub_spec e1 e2 (Binop Sub e1 e2).
+
+Lemma cp_subP e1 e2 : cp_sub_spec e1 e2 (cp_sub e1 e2).
+Proof.
+case: e1 => [x1|[|n1]|b1 e11 e12];
+case: e2 => [x2|[|n2]|b2 e21 e22];
+eauto using cp_sub_spec.
+Qed.
+
+Inductive cp_leq_spec : expr -> expr -> expr -> Prop :=
+| CpLeq1 n1 n2 : cp_leq_spec (Num n1) (Num n2) (Num (eval_binop Leq n1 n2))
+| CpLeq2 e : cp_leq_spec (Num 0) e (Num 1)
+| CpLeq3 e1 e2 : cp_leq_spec e1 e2 (Binop Leq e1 e2).
+
+Lemma cp_leqP e1 e2 : cp_leq_spec e1 e2 (cp_leq e1 e2).
+Proof.
+case: e1 => [x1|[|n1]|b1 e11 e12];
+case: e2 => [x2|[|n2]|b2 e21 e22];
+eauto using cp_leq_spec.
+Qed.
+
+Inductive cp_seq_spec : com -> com -> com -> Prop :=
+| CpSeq1 c : cp_seq_spec Skip c c
+| CpSeq2 c : cp_seq_spec c Skip c
+| CpSeq3 c1 c2 : cp_seq_spec c1 c2 (Seq c1 c2).
+
+Lemma cp_seqP c1 c2 : cp_seq_spec c1 c2 (cp_seq c1 c2).
+Proof.
+by case: c1 => *; case: c2 => *; eauto using cp_seq_spec.
+Qed.
+
+Inductive cp_assign_spec : string -> expr -> com -> Prop :=
+| CpAssign1 x : cp_assign_spec x (Var x) Skip
+| CpAssign2 x e : e ≠ Var x → cp_assign_spec x e (Assign x e).
+
+Lemma cp_assignP x e : cp_assign_spec x e (cp_assign x e).
+Proof.
+case: e => [y|n|b e1 e2]; eauto using cp_assign_spec.
+rewrite /= bool_decide_decide.
+case: (decide (x = y)) => [->|?]; eauto using cp_assign_spec.
+assert (Var y ≠ Var x) as ?. { congruence. }
+eauto using cp_assign_spec.
+Qed.
+
+Inductive cp_if_spec : expr -> com -> com -> com -> Prop :=
+| CPIf1 e c : cp_if_spec e c c c
+| CPIf2 c1 c2 : cp_if_spec (Num 0) c1 c2 c2
+| CPIf3 n c1 c2 : n ≠ 0 -> cp_if_spec (Num n) c1 c2 c1
+| CPIf4 e c1 c2 : cp_if_spec e c1 c2 (If e c1 c2).
+
+Lemma cp_ifP e c1 c2 : cp_if_spec e c1 c2 (cp_if e c1 c2).
+Proof.
+rewrite /cp_if. case: bool_decide_reflect => [<-|_]; first exact: CPIf1.
+case: e =>[x|[|n]|*]; eauto using cp_if_spec.
+Qed.
+
+Lemma eval_expr_notyet e s : eval_expr e s ≠ NotYet.
+Proof.
+elim: e => [x|n|b e1 IH1 e2 IH2] //=.
+- by case: (s !! x).
+- case: (eval_expr e1) => //= r1 in IH1 *.
+  case: (eval_expr e2) => //= r2 in IH2 *.
+Qed.
+
+Lemma result_bind_done {T} (x : result T) : mbind Done x = x.
+Proof. by case: x. Qed.
+
+Lemma result_bind_inv {A B} {f : A → result B} {x : result A} {y : B} :
+  (a ← x; f a) = Done y →
+  ∃ a, x = Done a ∧ f a = Done y.
+Proof.
+case: x => [x| | ] //=. eauto.
+Qed.
+
+Definition improves {T} (x y : result T) : Prop :=
+  y = Error ∨ x = y.
+
+Lemma improves_error {T} (x : result T) : improves x Error.
+Proof. by left. Qed.
+
+Lemma improves_refl {T} (x : result T) : improves x x.
+Proof. by right. Qed.
+
+Hint Resolve improves_error improves_refl : core.
+
+Lemma improves_trans {T} (x y z : result T) :
+  improves x y → improves y z → improves x z.
+Proof. by move=> H1 [->|<-]. Qed.
+
+Lemma improves_bind {T S} (x y : result T) (f g : T → result S) :
+  improves x y →
+  (∀ r, improves (f r) (g r)) →
+  improves (mbind f x) (mbind g y).
+Proof.
+case=> [->|->] //= f_g. by case: y => [r||] //=.
+Qed.
+
+Lemma improves_eval_expr {T} (x : result T) e s f :
+  (∀ n, improves x (f n)) →
+  improves x (mbind f (eval_expr e s)).
+Proof.
+have := eval_expr_notyet e s.
+case: eval_expr => //= n.
+Qed.
+
+Lemma cp_add_correct e1 e2 s :
+  eval_expr (cp_add e1 e2) s = eval_expr (Binop Add e1 e2) s.
+Proof.
+case: cp_addP => [n1 n2|e|e|{}e1 {}e2] //=.
+- by case: eval_expr => // n.
+- by case: eval_expr => //= n; rewrite Nat.add_0_r.
+Qed.
+
+Lemma cp_mul_correct e1 e2 s :
+  improves
+    (eval_expr (cp_mul e1 e2) s)
+    (eval_expr (Binop Mul e1 e2) s).
+Proof.
+rewrite /=.
+case: e1 e2 _ / cp_mulP => [n1 n2|e|e|e|e|e1 e2] //=.
+- by apply: improves_eval_expr.
+- by apply: improves_eval_expr => ?; rewrite Nat.mul_0_r.
+- rewrite -{1}[eval_expr e s]result_bind_done.
+  by apply: improves_bind => // n; rewrite Nat.add_0_r.
+- rewrite -{1}[eval_expr e s]result_bind_done.
+  by apply: improves_bind => // n; rewrite Nat.mul_1_r.
+Qed.
+
+Lemma cp_sub_correct e1 e2 s :
+  improves (eval_expr (cp_sub e1 e2) s) (eval_expr (Binop Sub e1 e2) s).
+Proof.
+rewrite /=.
+case: e1 e2 _ / cp_subP => [n1 n2|e|e|e1 e2] //=.
+- by apply: improves_eval_expr => ?; rewrite Nat.sub_0_l.
+- rewrite -{1}[eval_expr e s]result_bind_done.
+  by apply: improves_bind => // n; rewrite Nat.sub_0_r.
+Qed.
+
+Lemma cp_leq_correct e1 e2 s :
+  improves (eval_expr (cp_leq e1 e2) s) (eval_expr (Binop Leq e1 e2) s).
+Proof.
+rewrite /=; case: e1 e2 _ / cp_leqP => [n1' n2'|e|e1 e2] //=.
+by apply: improves_eval_expr.
+Qed.
+
+Lemma cp_binop_correct s b e1 e2 :
+  improves (eval_expr (cp_binop b e1 e2) s) (eval_expr (Binop b e1 e2) s).
+Proof.
+case: b.
+- by rewrite cp_add_correct.
+- exact: cp_mul_correct.
+- exact: cp_sub_correct.
+- exact: cp_leq_correct.
+Qed.
+
+Lemma cp_expr_correct e s :
+  improves (eval_expr (cp_expr e) s) (eval_expr e s).
+Proof.
+elim: e => [x|n'|b e1 IH1 e2 IH2] //=.
+apply: improves_trans.
+- exact: cp_binop_correct.
+- rewrite /=.
+  apply: improves_bind => // n1.
+  apply: improves_bind => // n2.
+Qed.
+Hint Resolve cp_expr_correct : core.
+
+Lemma cp_seq_correct c1 c2 s k :
+  improves (eval_com (cp_seq c1 c2) s k) (eval_com (Seq c1 c2) s k).
+Proof.
+case: c1 c2 _ / cp_seqP => [c|c|{}c1 c2] //=.
+rewrite -{1}[eval_com _ _ _]result_bind_done.
+by apply: improves_bind => //.
+Qed.
+
+Lemma cp_assign_correct x e s k :
+  improves (eval_com (cp_assign x e) s k) (eval_com (Assign x e) s k).
+Proof.
+case: x e _ / cp_assignP => [x|x e] //=.
+case E: (s !! x) => [n|] //=. by rewrite insert_id.
+Qed.
+
+Lemma cp_if_correct e c1 c2 s k :
+  improves (eval_com (cp_if e c1 c2) s k) (eval_com (If e c1 c2) s k).
+Proof.
+rewrite /=.
+case: e c1 c2 _ / cp_ifP=> [e c|c1 c2|n c1 c2 n_not_0|e c1 c2] //=.
+- apply: improves_eval_expr => //= n. by case: bool_decide.
+- by rewrite bool_decide_eq_false_2.
+Qed.
+
+Lemma cp_while_correct e c s k :
+  improves (eval_com (cp_while e c) s k) (eval_com (While e c) s k).
+Proof.
+rewrite /cp_while.
+case: bool_decide_reflect => [->|] //.
+by case: k.
+Qed.
+
+Lemma iter_improves {T} (f g : (T → result T) → T → result T) x k :
+  (∀ f' g', (∀ x, improves (f' x) (g' x)) →
+             ∀ x, improves (f f' x) (g g' x)) →
+  improves (iter f x k) (iter g x k).
+Proof.
+move=> H; elim: k => //= [|k IH] in x *; apply: H => // {}x.
+Qed.
+
+Lemma cp_com_correct c s k :
+  improves (eval_com (cp_com c) s k) (eval_com c s k).
+Proof.
+elim: c => [|c1 IH1 c2 IH2|x e|e c1 IH1 c2 IH2|e c IH] //= in s k *.
+- apply: improves_trans; first exact: cp_seq_correct.
+  by rewrite /=; apply: improves_bind => //.
+- apply: improves_trans; first exact: cp_assign_correct.
+  by rewrite /=; apply: improves_bind => //.
+- apply: improves_trans; first exact: cp_if_correct.
+  rewrite /=; apply: improves_bind => // n.
+  by case: bool_decide.
+- apply: improves_trans; first exact: cp_while_correct.
+  rewrite /=. apply: iter_improves=> f g f_g {}s.
+  apply: improves_bind => // - [|n] //=.
+  apply: improves_bind => //=.
+Qed.
